AP/AP/FreshA/Tile.lean
@@ -1,5 +1,10 @@
 import AP.AP.FreshA.CurrentTile
+import AP.AP.Moves
 
 namespace AP
+
+def AStrat.Fresh1A (a : AStrat) (s : State) (fsp : FSP) : Prop :=
+  s.aForallWinsDisj fsp a ∧ ∀ (d : DStrat), d.WF →
+  ∀ s₁ p, (s₁, p) ∈ s.aPtsSimAt ⟨a, d⟩ → p ∉ s.aVisited s₁
 
 -----
