AP/AP/Moves.lean
@@ -1,0 +1,326 @@
+import AP.AP.WF
+
+namespace AP
+
+def State.diff (s₁ s : State) : ℕ :=
+  s₁.hist.length - s.hist.length
+
+def State.diffTrs (s₁ s : State) : List PointZ :=
+  s₁.hist.take (s₁.diff s) |>.reverse
+
+def State.moveSim (s : State) (st : Strat) (s₁ : State) :
+Option # (PointZ × State) ⊕ (PointZ × State) := do
+  guard # (sys.simulate st.f s # s₁.diff s).1 = s₁
+  let p := st.f s₁
+  let s₂ ← sys.tr s₁ p
+  pure # ite s₁.aTurn Sum.inr Sum.inl (p, s₂)
+
+def State.aMoveSim (s : State) (st : Strat) (s₁ : State) : Option (PointZ × State) := do
+  match ← s.moveSim st s₁ with
+  | .inr r => some r
+  | _ => none
+
+def State.dMoveSim (s : State) (st : Strat) (s₁ : State) : Option (PointZ × State) := do
+  match ← s.moveSim st s₁ with
+  | .inl r => some r
+  | _ => none
+
+def State.aVisited' (s : State) (ps : List PointZ) : Set' PointZ :=
+  match ps with
+  | [] => ∅
+  | p :: ps =>
+    let set := sys.tr s p |>.iget.aVisited' ps
+    if s.aTurn then set.insert p else set
+
+def State.aVisited (s s₁ : State) : Set' PointZ :=
+  State.aVisited' s (s₁.diffTrs s) |>.insert s.aPos
+
+def State.aPtsSimAt (s : State) (st : Strat) : Set (State × PointZ) :=
+  {(s₁, p) | ∃ s₂, s.aMoveSim st s₁ = some (p, s₂)}
+
+def State.aPtsSim (s : State) (st : Strat) : Set PointZ :=
+  Prod.snd '' s.aPtsSimAt st
+
+-- #check 0 #exit
+
+-----
+
+theorem State.diff_eq_of_simulate' {s f n s₁ r}
+(h : sys.simulate f s n = (s₁, r)) : s₁.diff s + r = n := by
+  unfold diff
+  rw [length_hist_eq_of_simulate_eq h]
+  have h₁ := sys.snd_le_of_simulate_eq h
+  omega
+
+theorem State.diff_eq_of_simulate {s f n s₁ r}
+(h : sys.simulate f s n = (s₁, r)) : s₁.diff s = n - r := by
+  have := diff_eq_of_simulate' h; omega
+
+theorem State.diff_eq_of_simulate_full {s f n s₁}
+(h : sys.simulate f s n = (s₁, 0)) : s₁.diff s = n :=
+  diff_eq_of_simulate h
+
+@[simp]
+theorem State.length_diffTrs {s s₁ : State} : (s₁.diffTrs s).length = s₁.diff s := by
+  simp [diffTrs, diff]
+
+@[simp]
+theorem State.diff_self {s : State} : s.diff s = 0 := by
+  simp [diff]
+
+@[simp]
+theorem State.diffTrs_self {s : State} : s.diffTrs s = [] := by
+  simp [diffTrs]
+
+@[simp]
+theorem State.aVisited'_nil {s : State} : s.aVisited' [] = ∅ := rfl
+
+@[simp]
+theorem State.aVisited_self {s : State} : s.aVisited s = Set'.singleton s.aPos := by
+  simp [aVisited]
+
+theorem State.diff_eq_of_tr {s s₁ s₂ p} (h : sys.tr s₁ p = some s₂)
+(h₁ : sys.Reachable s s₁) : s₂.diff s = s₁.diff s + 1 := by
+  simp [diff, length_hist_eq_of_tr h]; have := length_hist_le_of_reachable h₁; omega
+
+theorem State.diffTrs_eq_of_tr {s s₁ s₂ p} (h : sys.tr s₁ p = some s₂)
+(h₁ : sys.Reachable s s₁) : s₂.diffTrs s = s₁.diffTrs s ++ [p] := by
+  simp [diffTrs, diff_eq_of_tr h h₁, hist_eq_of_tr h]
+
+theorem State.diffTrs_eq_of_trs_full {s ps s₁}
+(h : sys.trs s ps = (s₁, [])) : s₁.diffTrs s = ps := by
+  induction ps using List.reverseRecOn generalizing s₁
+  · simp at h; simp [h]
+  nm ps p ih
+  simp at h
+  choose s' h₁ h₂ using h
+  specialize ih h₁
+  simpa [diffTrs_eq_of_tr h₂ # sys.reachable_of_trs h₁]
+
+@[simp]
+theorem State.aVisited'_singleton {s : State} {p} :
+s.aVisited' [p] = if s.aTurn then Set'.singleton p else ∅ := by
+  simp [aVisited']
+
+theorem AState.aVisited'_cons {s s' : State} {p ps} [hs : AState s]
+(h : sys.tr s p = some s') : s.aVisited' (p :: ps) =
+(s'.aVisited' ps).insert p := by
+  simp [State.aVisited', h]
+
+theorem DState.aVisited'_cons {s s' : State} {p ps} [hs : DState s]
+(h : sys.tr s p = some s') : s.aVisited' (p :: ps) = s'.aVisited' ps := by
+  simp [State.aVisited', h]
+
+theorem AState.aVisited'_snoc {s s₁ : State} {ps p} [hs : sys.WF s]
+[hs₁ : AState s₁] (h₁ : sys.trs s ps = (s₁, [])) :
+s.aVisited' (ps ++ [p]) = (s.aVisited' ps).insert p := by
+  induction ps generalizing s
+  · simp at h₁; simp [h₁]
+  nm p₁ ps ih
+  simp at h₁
+  choose s' h₁ h₃ using h₁
+  have hs' := sys.wf_of_tr h₁
+  specialize ih h₃
+  replace hs := s.aState_or_dState
+  rw [List.cons_append]
+  rcases hs with hs | hs
+  · simp_rw [AState.aVisited'_cons h₁, ih, Set'.insert_comm]
+  · simp_rw [DState.aVisited'_cons h₁, ih]
+
+theorem DState.aVisited'_snoc {s s₁ : State} {ps p} [hs : sys.WF s]
+[hs₁ : DState s₁] (h₁ : sys.trs s ps = (s₁, [])) :
+s.aVisited' (ps ++ [p]) = s.aVisited' ps := by
+  induction ps generalizing s
+  · simp at h₁; simp [h₁]
+  nm p₁ ps ih
+  simp at h₁
+  choose s' h₁ h₃ using h₁
+  have hs' := sys.wf_of_tr h₁
+  specialize ih h₃
+  replace hs := s.aState_or_dState
+  rw [List.cons_append]
+  rcases hs with hs | hs
+  · simp_rw [AState.aVisited'_cons h₁, ih]
+  · simp_rw [DState.aVisited'_cons h₁, ih]
+
+theorem AState.aVisited_eq_of_tr {s s₁ s₂ p} [hs : sys.WF s] [hs₁ : AState s₁]
+(h : sys.tr s₁ p = some s₂) (h₁ : sys.Reachable s s₁) :
+s.aVisited s₂ = (s.aVisited s₁).insert p := by
+  rw [sys.reachable_iff_exi_trs] at h₁
+  choose ps h₁ using h₁
+  simp [State.aVisited]
+  rw [State.diffTrs_eq_of_trs_full h₁]
+  have h₂ : sys.trs s (ps ++ [p]) = (s₂, [])
+  · simpa [h₁]
+  rw [State.diffTrs_eq_of_trs_full h₂, Set'.insert_comm]
+  rw [aVisited'_snoc h₁]
+
+theorem DState.aVisited_eq_of_tr {s s₁ s₂ p} [hs : sys.WF s] [hs₁ : DState s₁]
+(h : sys.tr s₁ p = some s₂) (h₁ : sys.Reachable s s₁) :
+s.aVisited s₂ = s.aVisited s₁ := by
+  rw [sys.reachable_iff_exi_trs] at h₁
+  choose ps h₁ using h₁
+  simp [State.aVisited]
+  rw [State.diffTrs_eq_of_trs_full h₁]
+  have h₂ : sys.trs s (ps ++ [p]) = (s₂, [])
+  · simpa [h₁]
+  rw [State.diffTrs_eq_of_trs_full h₂]
+  rw [aVisited'_snoc h₁]
+
+theorem State.mem_aVisited_iff {s f n s₁ p} [hs : sys.WF s]
+(h : sys.simulate f s n = (s₁, 0)) : p ∈ s.aVisited s₁ ↔ p = s.aPos ∨
+∃ k < n, ∃ s', AState s' ∧ sys.simulate f s k = (s', 0) ∧ f s' = p := by
+  induction n generalizing s₁
+  · simp at h; simp [h]
+  nm n ih
+  rw [sys.simulate_succ_full'] at h
+  choose s' h₁ h₂ using h
+  specialize ih h₁
+  have hs' : sys.WF s' := sys.wf_of_simulate_eq h₁
+  have hs₁ := sys.wf_of_tr h₂
+  have h₃ := sys.reachable_of_simulate_eq h₁
+  replace hs' := s'.aState_or_dState
+  rcases hs' with hs' | hs'
+  all_goals simp [hs'.aVisited_eq_of_tr h₂ h₃, ih]; clear ih
+  · grind
+  apply iff_of_eq; congr 1; apply propext
+  apply exists_congr; intro k
+  rw [Nat.lt_add_one_iff]
+  by_cases h : k ≠ n
+  · simp [le_iff_eq_or_lt, h]
+  push_neg at h; subst h
+  simp
+  rintro s₂ hs₂ h₄ rfl
+  simp [h₁] at h₄
+  contrapose! h₄
+  apply ne_of_congr (·.aTurn); simp
+
+theorem State.trs_diffTrs {s s₁ ps ps'} [hs : sys.WF s]
+(h : sys.trs s ps = (s₁, ps')) : sys.trs s (s₁.diffTrs s) = (s₁, []) := by
+  induction ps using List.reverseRecOn generalizing s s₁ ps'
+  · simp at h; simp [h]
+  nm ps p ih
+  simp [sys.trs_append] at h
+  generalize hr : sys.trs s ps = r at h
+  rcases r with ⟨s', r⟩
+  dsimp at h
+  split_ifs at h with h₁
+  · subst h₁
+    simp at h
+    specialize ih hr
+    simp [System.trs] at h
+    split at h
+    · grind
+    nm x s₂ h₁; clear x
+    simp at h
+    rcases h with ⟨rfl, rfl⟩
+    rw [diffTrs_eq_of_tr h₁ # sys.reachable_of_trs hr]
+    simpa [ih]
+  simp at h
+  rcases h with ⟨rfl, rfl⟩
+  exact ih hr
+
+theorem State.simulate_diff {s s₁ f n r} [hs : sys.WF s]
+(h : sys.simulate f s n = (s₁, r)) : sys.simulate f s (s₁.diff s) = (s₁, 0) := by
+  induction n generalizing s s₁ r
+  · simp at h; simp [h]
+  nm n ih
+  rw [sys.simulate_add] at h
+  simp at h
+  generalize hr : sys.simulate f s n = r at h
+  rcases r with ⟨s', r⟩
+  dsimp at h
+  split_ifs at h with h₁
+  · subst h₁
+    simp at h
+    specialize ih hr
+    simp [System.simulate] at h
+    split at h
+    · grind
+    nm x s₂ h₁; clear x
+    simp at h
+    rcases h with ⟨rfl, rfl⟩
+    rw [diff_eq_of_tr h₁ # sys.reachable_of_simulate_eq hr]
+    rw [sys.simulate_add]
+    simpa [ih]
+  simp at h
+  rcases h with ⟨rfl, rfl⟩
+  exact ih hr
+
+theorem State.aPtsSim_eq_setOf {s : State} {st} : s.aPtsSim st =
+{p | ∃ s₁ s₂, s.aMoveSim st s₁ = some (p, s₂)} := by
+  ext; simp [aPtsSim, aPtsSimAt]
+
+theorem State.mem_aPtsSim_iff_aPtsSimAt {s : State} {st p} :
+p ∈ s.aPtsSim st ↔ ∃ s₁, (s₁, p) ∈ s.aPtsSimAt st := by
+  simp [aPtsSim]
+
+theorem State.mem_aPtsSimAt_iff_simulate_tr {s s₁ p} {st : Strat} [hs : sys.WF s] :
+(s₁, p) ∈ s.aPtsSimAt st ↔ AState s₁ ∧ ∃ n, sys.simulate st.f s n = (s₁, 0) ∧
+∃ s₂, sys.tr s₁ (st.a.f s₁) = some s₂ ∧ st.a.f s₁ = p := by
+  simp only [aPtsSimAt, aMoveSim, moveSim, Option.pure_def, Option.bind_eq_bind,
+    Option.bind_eq_some_iff', Option.guard_eq_some', Option.some.injEq, exists_const, Sum.exists,
+    reduceCtorEq, and_false, exists_eq_right, false_or, exists_and_left, Set.mem_setOf_eq,
+    exists_and_right]
+  constructor
+  · rintro ⟨h₁, s₂, s₃, h₂, h₃⟩
+    split_ifs at h₃ with ht
+    simp at h₃
+    rcases h₃ with ⟨rfl, rfl⟩
+    apply and_of
+    · constructor
+      · rw [←h₁]; infer_instance
+      exact ht
+    intro hs₁
+    clear ht
+    simp
+    generalize hr : sys.simulate st.f s (s₁.diff s) = r at h₁ ⊢
+    rcases r with ⟨s₁, r⟩
+    dsimp at *
+    subst h₁
+    simp at h₂ ⊢
+    simp [h₂]
+    use s₁.diff s - r, sys.simulate_sub_eq_of hr
+  · rintro ⟨hs₁, ⟨n, h₁⟩, ⟨s₂, h₂⟩, rfl⟩
+    simp [simulate_diff h₁]
+    use s₂
+
+theorem State.mem_aPtsSim_iff_simulate_tr {s p} {st : Strat} [hs : sys.WF s] :
+p ∈ s.aPtsSim st ↔ ∃ n s₁, AState s₁ ∧ sys.simulate st.f s n = (s₁, 0) ∧
+∃ s₂, sys.tr s₁ (st.a.f s₁) = some s₂ ∧ st.a.f s₁ = p := by
+  simp_rw [mem_aPtsSim_iff_aPtsSimAt, mem_aPtsSimAt_iff_simulate_tr]; grind
+
+theorem State.mem_aPtsSim_iff_simulate_ge_two {s p} {st : Strat} [hst : st.WF] [hs : sys.WF s] :
+p ∈ s.aPtsSim st ↔ ∃ n s₁, 2 ≤ n ∧ sys.simulate st.f s n = (s₁, 0) ∧ s₁.aPos = p := by
+  rw [mem_aPtsSim_iff_simulate_tr]
+  constructor
+  · rintro ⟨n, s₁, hs₁, h₁, s₂, h₂, rfl⟩
+    have hs₂ := DState.of_tr h₂
+    obtain ⟨s₃, h₃⟩ : sys.validTr s₂ (st.d.f s₂)
+    · simp
+    use n + 2, by omega
+    rw [sys.simulate_add]
+    simp [System.simulate, h₁, h₂, h₃]
+    rw [DState.aPos_eq_of_tr h₃, AState.aPos_eq_of_tr h₂]
+  · rintro ⟨n, s₃, hn, h₁, rfl⟩
+    simp only [exists_and_right]
+    obtain ⟨n, rfl⟩ := Nat.exists_eq_add_of_le hn; clear hn
+    rw [add_comm] at h₁
+    simp_rw [sys.simulate_succ_full'] at h₁
+    obtain ⟨s₂, ⟨s₁, h₁, h₂⟩, h₃⟩ := h₁
+    have hs₁ : sys.WF s₁ := sys.wf_of_simulate_eq h₁
+    replace hs₁ := s₁.aState_or_dState
+    rcases hs₁ with hs₁ | hs₁
+    · simp at h₂
+      have hs₂ := DState.of_tr h₂
+      use n, s₁, hs₁, h₁
+      refine ⟨⟨s₂, h₂⟩, ?_⟩
+      rw [DState.aPos_eq_of_tr h₃, AState.aPos_eq_of_tr h₂]
+    · have hs₂ := AState.of_tr h₂
+      simp at h₂ h₃
+      use n + 1, s₂, hs₂
+      rw [sys.simulate_add]
+      simp [h₁]
+      use h₂
+      refine ⟨⟨s₃, h₃⟩, ?_⟩
+      rw [AState.aPos_eq_of_tr h₃]
