AP/AP/WF.lean
@@ -211,7 +211,7 @@ theorem State.exi_hist_wf_of_wfCnd {s} (h : WFCnd s) : ∃ hist, sys.WF # s.setH
     split_ands
     · rintro rfl; exact h.aPos_not_mem_taken hp
     ext:1 <;> simp [ht]
-    rw [Set'.eq_insert_empty_of_size_eq_one h₃ hp]
+    simp [Set'.eq_insert_empty_of_size_eq_one h₃ hp]
   have H₁ := h.aPos_not_mem_taken
   by_cases h₁ : ∃ p, p ∈ s.taken ∧ p.dist s.aPos ≤ s.pw
   · obtain ⟨p, hp, h₁⟩ := h₁
